Deleted some unnecessary functions and lemmas

Sequences.dfy
@@ -29,17 +29,17 @@ module Seq {
   }
 
   // returns the last element in the sequence
-  function method last<E>(run: seq<E>): E
-    requires |run| > 0;
+  function method last<E>(s: seq<E>): E
+    requires |s| > 0;
   {
-    run[|run|-1]
+    s[|s|-1]
   }
 
   // returns the sequence slice up to but not including the last element
-  function method drop_last<E>(run: seq<E>): seq<E> 
-  requires |run| > 0;
+  function method drop_last<E>(s: seq<E>): seq<E> 
+  requires |s| > 0;
   {
-    run[..|run|-1]
+    s[..|s|-1]
   }
 
   // concatenating everything but the last element + the last element results in the original seq 
@@ -51,30 +51,30 @@ module Seq {
   }
   
   // converts a sequence to a multiset
-  function method to_set<T>(run: seq<T>): set<T> 
+  function method to_set<T>(s: seq<T>): set<T> 
   {
-    set x: T | x in multiset(run)
+    set x: T | x in multiset(s)
   }
 
 
   /* proves that the cardinality of a subsequence is always less than or equal to that
   of the full sequence */
-  lemma lemma_cardinality_of_set<T>(run: seq<T>)
-    ensures |to_set(run)| <= |run| // length of the subset is less than the length of the set
+  lemma lemma_cardinality_of_set<T>(s: seq<T>)
+    ensures |to_set(s)| <= |s| // length of the subset is less than the length of the set
   {
-    if |run| == 0 {
+    if |s| == 0 {
     } else {
-      assert to_set(run) == to_set(drop_last(run)) + {last(run)};
-      lemma_cardinality_of_set(drop_last(run));
+      assert to_set(s) == to_set(drop_last(s)) + {last(s)};
+      lemma_cardinality_of_set(drop_last(s));
     }
   }
   
   // the cardinality of a subsequence of an empty sequence is also 0
-  lemma lemma_cardinality_of_empty_set_is_0<T>(run: seq<T>)
-    ensures |to_set(run)| == 0 <==> |run| == 0
+  lemma lemma_cardinality_of_empty_set_is_0<T>(s: seq<T>)
+    ensures |to_set(s)| == 0 <==> |s| == 0
   {
-    if |run| != 0 {
-      assert run[0] in to_set(run);
+    if |s| != 0 {
+      assert s[0] in to_set(s);
     }
   }
 
@@ -158,37 +158,37 @@ module Seq {
   }
 
   // applies a transformation function on the sequence
-  function method {:opaque} Map<E,R>(f: (E ~> R), run: seq<E>): (result: seq<R>)
-    requires forall i :: 0 <= i < |run| ==> f.requires(run[i])
-    ensures |result| == |run|
-    ensures forall i :: 0 <= i < |run| ==> result[i] == f(run[i]);
-    reads set i, o | 0 <= i < |run| && o in f.reads(run[i]):: o
+  function method {:opaque} Map<E,R>(f: (E ~> R), s: seq<E>): (result: seq<R>)
+    requires forall i :: 0 <= i < |s| ==> f.requires(s[i])
+    ensures |result| == |s|
+    ensures forall i :: 0 <= i < |s| ==> result[i] == f(s[i]);
+    reads set i, o | 0 <= i < |s| && o in f.reads(s[i]):: o
   {
-    if |run| == 0 then []
-    else  [f(run[0])] + Map(f, run[1..])
+    if |s| == 0 then []
+    else  [f(s[0])] + Map(f, s[1..])
   }
 
   // uses a selection function to select elements from the sequence
-  function method filter<E>(f : (E ~> bool), run: seq<E>): (result: seq<E>)
-    requires forall i :: 0 <= i < |run| ==> f.requires(run[i])
-    ensures |result| <= |run|
+  function method {:opaque} filter<E>(f : (E ~> bool), s: seq<E>): (result: seq<E>)
+    requires forall i :: 0 <= i < |s| ==> f.requires(s[i])
+    ensures |result| <= |s|
     ensures forall i: nat :: i < |result| && f.requires(result[i]) ==> f(result[i])
     reads f.reads
   {
-    if |run| == 0 then []
-    else ((if f(run[0]) then [run[0]] else []) + filter(f, run[1..]))
+    if |s| == 0 then []
+    else ((if f(s[0]) then [s[0]] else []) + filter(f, s[1..]))
   }
   
-  function method fold_left<A,E>(f: (A, E) -> A, init: A, run: seq<E>): A
+  function method {:opaque} fold_left<A,E>(f: (A, E) -> A, init: A, s: seq<E>): A
   {
-    if |run| == 0 then init
-    else fold_left(f, f(init, run[0]), run[1..])
+    if |s| == 0 then init
+    else fold_left(f, f(init, s[0]), s[1..])
   }
 
-  function method fold_right<A,E>(f: (A, E) -> A, init: A, run: seq<E>): A
+  function method {:opaque} fold_right<A,E>(f: (A, E) -> A, init: A, s: seq<E>): A
   {
-    if |run| == 0 then init
-    else f(fold_right(f, init, run[1..]), run[0])
+    if |s| == 0 then init
+    else f(fold_right(f, init, s[1..]), s[0])
   }
 
   // slices out a specific position's value from the sequence and returns the new sequence
@@ -408,17 +408,6 @@ module Seq {
       [v] + repeat(v, length - 1)
   }
 
-  // This is a workaround since Dafny right now doesn't support
-  // s[i := t] when i is a native type integer.
-  //already a function method
-  function method {:opaque} SeqIndexUpdate<T>(s: seq<T>, i: int, t: T): seq<T>
-  requires i as int + 1 < 0x1_0000_0000_0000_0000
-  requires 0 <= i as int < |s|
-  ensures SeqIndexUpdate(s, i, t) == s[i as int := t]
-  {
-    s[..i] + [t] + s[i+1..]
-  }
-
   /* takes two sequences, a and b, and combines then to form one sequence in which
   each position contains an ordered pair from a and b */
   function method {:opaque} zip<A,B>(a: seq<A>, b: seq<B>): seq<(A,B)>
@@ -454,232 +443,6 @@ module Seq {
     ensures unzip(zip(sa, sb)).1 == sb
   {
   }
-  
-  /* receives a sequence of sequences. Returns a sequence in which the ith element corresponds 
-  to the length of the sequence at the ith position*/
-  function method {:opaque} flatten_shape<A>(seqs: seq<seq<A>>): (shape: seq<nat>)
-    ensures |shape| == |seqs|
-    ensures forall i :: 0 <= i < |shape| ==> shape[i] == |seqs[i]|
-  {
-    if |seqs| == 0 then []
-    else flatten_shape(drop_last(seqs)) + [|last(seqs)|]
-  }
-
-  /* concatenating two sequences and then flattening their shape retults in the same
-  result as flattenning each sequence first and then concatenating */
-  lemma lemma_flatten_shape_addition<A>(seqs1: seq<seq<A>>, seqs2: seq<seq<A>>)
-    ensures flatten_shape(seqs1 + seqs2) == flatten_shape(seqs1) + flatten_shape(seqs2)
-  {
-  }
-  
-  /* returns a number that results from adding up each all 
-  of the elements in the sequence's shape */
-  function method {:opaque} flatten_length(shape: seq<nat>): nat
-    ensures |shape| == 0 ==> flatten_length(shape) == 0
-  {
-    if |shape| == 0 then 0
-    else flatten_length(drop_last(shape)) + last(shape)
-  }
-
-  /* concatenating two "shape" sequences together and then flattening their length is 
-  the same as flattening each shape's length and then adding the resulting numbers */
-  lemma {:induction true} lemma_flatten_length_addition(shape1: seq<nat>, shape2: seq<nat>)
-    ensures flatten_length(shape1 + shape2) == flatten_length(shape1) + flatten_length(shape2)
-  {
-    if |shape2| == 0 {
-      assert shape1 + shape2 == shape1;
-    } else {
-      reveal_flatten_length();
-      assert shape1 + shape2 == (shape1 + drop_last(shape2)) + [last(shape2)];
-    }
-  }
-  
-  /* the flattened length of any subsequence of the shape is less than 
-  the flattened length of the whole shape */
-  lemma lemma_flatten_length_subseq(shape: seq<nat>, from: nat, to: nat)
-    requires from <= to <= |shape|
-    ensures flatten_length(shape[from..to]) <= flatten_length(shape)
-  {
-    assert shape == shape[..from] + shape[from..to] + shape[to..];
-    lemma_flatten_length_addition(shape[..from] + shape[from..to], shape[to..]);
-    lemma_flatten_length_addition(shape[..from], shape[from..to]);
-  }
-
-  /* the flattened sequence's length will be equal to flattenening the shape 
-  and then flattening the length; returns a sequence that combines all sequences of 
-  the sequence */
-  function method {:opaque} flatten<A>(seqs: seq<seq<A>>): seq<A>
-    ensures |flatten(seqs)| == flatten_length(flatten_shape(seqs))
-    ensures |seqs| == 0 ==> |flatten(seqs)| == 0
-  {
-    reveal_flatten_shape();
-    reveal_flatten_length();
-    if |seqs| == 0 then []
-    else flatten(drop_last(seqs)) + last(seqs)
-  }
-
-  // flattening a singleton of sequences will simply result in the original sequence
-  lemma lemma_flatten_singleton<A>(s: seq<A>)
-    ensures flatten([ s ]) == s
-  {
-    reveal_flatten();
-  }
-  
-  /* concatenating two sequences and then flattening them has the same result 
-  as flattening each sequence seperately and then concatenating afterwards */
-  lemma lemma_flatten_addition<A>(seqs1: seq<seq<A>>, seqs2: seq<seq<A>>)
-    ensures flatten(seqs1 + seqs2) == flatten(seqs1) + flatten(seqs2)
-    decreases |seqs2|
-  {
-    if |seqs2| == 0 {
-      assert seqs1 + seqs2 == seqs1;
-    } else if |seqs2| == 1 {
-      reveal_flatten();
-    } else {
-      calc {
-        flatten(seqs1 + seqs2);
-        { assert seqs1 + seqs2 == seqs1 + drop_last(seqs2) + [ last(seqs2) ]; }
-        flatten(seqs1 + drop_last(seqs2) + [ last(seqs2) ]);
-        { lemma_flatten_addition(seqs1 + drop_last(seqs2), [ last(seqs2) ]); }
-        flatten(seqs1 + drop_last(seqs2)) + flatten([ last(seqs2) ]);
-        { lemma_flatten_addition(seqs1, drop_last(seqs2)); }
-        flatten(seqs1) + flatten(drop_last(seqs2)) + flatten([ last(seqs2) ]);
-        { lemma_flatten_addition(drop_last(seqs2), [ last(seqs2) ]); }
-        flatten(seqs1) + flatten(drop_last(seqs2) + [ last(seqs2) ]);
-        { assert seqs2 == drop_last(seqs2) + [ last(seqs2) ]; }
-        flatten(seqs1) + flatten(seqs2);
-      }
-    }
-  }
-  
-  /* returns the index of the flattened sequence  */
-  function method flatten_index(shape: seq<nat>, i: nat, j: nat): nat
-    requires i < |shape|
-    requires j < shape[i]
-  {
-    flatten_length(shape[..i]) + j
-  }
-
-  /* returns the index of the unflattened sequence */
-  function method unflatten_index(shape: seq<nat>, i: nat): (nat, nat)
-    requires i < flatten_length(shape)
-  {
-    reveal_flatten_length();
-    if i < flatten_length(drop_last(shape)) then unflatten_index(drop_last(shape), i)
-    else (|shape|-1, i - flatten_length(drop_last(shape)))
-  }
-
-  /* the index in a flattened sequence is less than the flattened length
-  of the entire sequence */
-  lemma lemma_flatten_index_in_bounds(shape: seq<nat>, i: nat, j: nat)
-    requires i < |shape|
-    requires j < shape[i]
-    ensures flatten_index(shape, i, j) < flatten_length(shape)
-  {
-    reveal_flatten_length();
-    if i == |shape|-1 {
-    } else {
-      lemma_flatten_index_in_bounds(drop_last(shape), i, j);
-      assert drop_last(shape)[..i] == shape[..i];
-    }
-  }
-  
-  /* the unflattened index is in the bounds if the index is less than the sequence's flattened length  */
-  lemma {:induction true} lemma_unflatten_index_in_bounds(shape: seq<nat>, i: nat)
-    requires i < flatten_length(shape)
-    ensures unflatten_index(shape, i).0 < |shape|
-    ensures unflatten_index(shape, i).1 < shape[unflatten_index(shape, i).0]
-  {
-    var shapeidx := unflatten_index(shape, i).0;
-  }
-
-  /* flattening and then unflattening the sequence results in the original sequence */
-  lemma {:induction true} lemma_flatten_unflatten_indentity(shape: seq<nat>, i: nat)
-    requires i < flatten_length(shape)
-    ensures unflatten_index(shape, i).0 < |shape|
-    ensures unflatten_index(shape, i).1 < shape[unflatten_index(shape, i).0]
-    ensures i == flatten_index(shape, unflatten_index(shape, i).0, unflatten_index(shape, i).1)
-  {
-    lemma_unflatten_index_in_bounds(shape, i);
-    var (shapeidx, shapeoff):= unflatten_index(shape, i);
-    if shapeidx == |shape|-1 {
-    } else {
-      lemma_flatten_unflatten_indentity(drop_last(shape), i);
-      assert drop_last(shape)[..shapeidx] == shape[..shapeidx];
-    }
-  }
-  
-  /* unflattening and then flattening the sequence results in the original sequence */
-  lemma lemma_unflatten_flatten_identity(shape: seq<nat>, i: nat, j: nat)
-    requires i < |shape|
-    requires j < shape[i]
-    ensures flatten_index(shape, i, j) < flatten_length(shape)
-    ensures (i, j) == unflatten_index(shape, flatten_index(shape, i, j))
-  {
-    lemma_flatten_index_in_bounds(shape, i, j);
-    if i == |shape| - 1 {
-    } else {
-      lemma_unflatten_flatten_identity(drop_last(shape), i, j);
-      assert drop_last(shape)[..i] == shape[..i];
-    }
-  }
-  
-  // the ordering of flattened indicies is also an indicator of placement in the unflattened sequence
-  lemma {:induction true} lemma_unflatten_index_ordering(shape: seq<nat>, i: nat, j: nat)
-    requires i < j < flatten_length(shape)
-    ensures unflatten_index(shape, i).0 <= unflatten_index(shape, j).0
-    ensures unflatten_index(shape, i).0 == unflatten_index(shape, j).0 ==> unflatten_index(shape, i).1 < unflatten_index(shape, j).1
-  {
-    lemma_flatten_unflatten_indentity(shape, i);
-  }
-
-  // the flattened index is correct
-  lemma lemma_flatten_index_is_correct<A>(seqs: seq<seq<A>>, i: nat, j: nat)
-    requires i < |seqs|
-    requires j < |seqs[i]|
-    ensures flatten_index(flatten_shape(seqs), i, j) < |flatten(seqs)|
-    ensures flatten(seqs)[flatten_index(flatten_shape(seqs), i, j)] == seqs[i][j]
-  {
-    reveal_flatten();
-    lemma_flatten_index_in_bounds(flatten_shape(seqs), i, j);
-    if i == |seqs|-1 {
-    } else {
-      lemma_flatten_index_is_correct(drop_last(seqs), i, j);
-      assert drop_last(flatten_shape(seqs))[..i] == flatten_shape(seqs)[..i];
-    }
-  }
-
-  // proves that the unflattened index is correct
-  lemma {:induction true} {:timeLimitMultiplier 3} lemma_unflatten_index_is_correct<A>(seqs: seq<seq<A>>, i: nat)
-    requires i < flatten_length(flatten_shape(seqs))
-    ensures unflatten_index(flatten_shape(seqs), i).0 < |seqs|
-    ensures unflatten_index(flatten_shape(seqs), i).1 < |seqs[unflatten_index(flatten_shape(seqs), i).0]|
-    ensures flatten(seqs)[i] == seqs[unflatten_index(flatten_shape(seqs), i).0][unflatten_index(flatten_shape(seqs), i).1]
-  {
-    var shape := flatten_shape(seqs);
-    lemma_unflatten_index_in_bounds(shape, i);
-    reveal_flatten();
-  }
-
-  /* proves that the cardinality of the set is the same as the cardinality 
-  of the sequence, given that the set is the same size as the sequence*/
-  lemma lemma_cardinality_of_set_and_sequence<T>(q:seq<T>, t:set<int>)
-    requires t == set i | 0 <= i < |q|
-    ensures |t| == |q|
-  {
-    if |q| > 0 {
-      var sq := q[..|q|-1];
-      var st := set i | 0 <= i < |sq|;
-      calc {
-        |q|;
-        |sq| + 1;
-          { lemma_cardinality_of_set_and_sequence(sq, st); }
-        |st| + 1;
-          { assert t == st + {|sq|}; }
-        |t|;
-      }
-    }
-  }
 
   // returns the maximum integer value in the sequence
   function method {:opaque} seq_max(s: seq<int>): int
@@ -693,23 +456,6 @@ module Seq {
       s[0]
     else
       Math.max(seq_max(drop_last(s)), last(s))
-  }
-
-  /* the maximum value in sequence 1 is greater than or equal to the maximum
-  value of sequence 2 */
-  lemma lemma_seq_max_correspondence(s1:seq<int>, s2:seq<int>, wit: seq<nat>)
-    requires 0 < |s1|
-    requires 0 < |s2|
-    requires |wit| == |s2|
-    requires forall j:nat :: j < |wit| ==> wit[j] < |s1|
-    requires forall i :: 0 <= i < |s2| ==> s2[i] <= s1[wit[i]]
-    ensures seq_max(s2) <= seq_max(s1)
-  {
-    if seq_max(s2) > seq_max(s1) {
-      var idx :| 0 <= idx < |s2| && s2[idx] == seq_max(s2);
-      assert s1[wit[idx]] in s1;  // trigger
-      assert false;
-    }
   }
 
   /* the maximum element in any subsequence will not be 
@@ -729,94 +475,6 @@ module Seq {
     requires a <= pos < b;
     ensures  0 <= pos - a < |s'|;
     ensures  s'[pos-a] == s[pos];
-  {
-  }
-
-  /* proves that if a sequence is sliced from i until the end and then sliced a seconds time, 
-  the resulting sequence is the same as the original sequence shifted by i */ 
-  lemma lemma_seq_suffix_slice<T>(s: seq<T>, i: int, j: int, k: int)
-    requires 0 <= i <= |s|
-    requires 0 <= j <= k <= |s| - i
-    ensures s[i..][j..k] == s[i+j..i+k];
-  {
-  }
-
-  // the given element is included in the sequence's sliced portion
-  lemma lemma_element_from_seq_suffix<T>(s: seq<T>, s':seq<T>, a:int, pos:int)
-    requires 0 <= a <= |s|;
-    requires s' == s[a..];
-    requires a <= pos < |s|;
-    ensures  s'[pos-a] == s[pos];
-  {
-  }
-
-  /* if a sequence is sliced after the a certain length, the new sequence's
-  elements' values are shifted down by that length*/
-  lemma lemma_seq_suffix<T>(s: seq<T>, prefix_length: int, index: int)
-    requires 0 <= prefix_length <= index < |s|;
-    ensures s[index] == s[prefix_length..][index - prefix_length];
-  {
-  }
-
-  /* if a sequence is sliced in a certain interval and then sliced again
-  from k until the end, then this is the same as slicing the initial
-  sequence from the first + the second slice */
-  lemma lemma_seq_slice_suffix<T>(s: seq<T>, i: int, j: int, k: int)
-    requires 0 <= i <= j <= |s|
-    requires 0 <= k <= j - i
-    ensures s[i..j][k..] == s[i+k..j];
-  { 
-  }
-
-  /* proves that if an array is sliced from i until the end and then sliced a seconds time, 
-  the resulting array is the same as the original array shifted by i */ 
-  lemma lemma_array_suffix_slice<T>(ar: array<T>, i: int, j: int, k: int)
-    requires 0 <= i <= ar.Length
-    requires 0 <= j <= k <= ar.Length - i
-    ensures ar[i..][j..k] == ar[i+j..i+k];
-  {
-  }
-
-  /* if a sequence is sliced after the first element, the new sequence's
-  elements' values are shifted down by 1 */
-  lemma lemma_seq_shift_after_slicing<T>(sequence:seq<T>, j:int)
-    requires 0<=j<|sequence|-1;
-    ensures sequence[1..][j] == sequence[j+1];
-  {
-  }
-
-  // increments all of the elements of the sequence of ints by a specified amount
-  function method increment_seq(s: seq<int>, amount:int): seq<int>
-    ensures var s' := increment_seq(s, amount);
-      |s| == |s'| && forall i :: 0 <= i < |s'| ==> s'[i] == s[i] + amount;
-  {
-    if s == [] then [] else [s[0] + amount] + increment_seq(s[1..], amount)
-  }
-
-  // proves that sequence a and b are equal
-  lemma lemma_seq_equal<E>(a: seq<E>, b: seq<E>)
-    requires |a| == |b|
-    requires forall i :: 0 <= i < |a| ==> a[i] == b[i]
-    ensures a == b
-  {
-  }
-
-  /* if sequence a and sequence b are of equall lengths and all of their
-  elements are equal, a and b are equal sequences */ 
-  lemma lemma_seq_equality<T>(a:seq<T>, b:seq<T>, len:int)
-    requires |a| == |b| == len;
-    requires forall i {:trigger a[i]}{:trigger b[i]} :: 0 <= i < len ==> a[i] == b[i];
-    ensures a == b;
-  {
-    assert forall i :: 0 <= i < len ==> a[i] == b[i];
-  }
-
-  /* if the length two sequences are equal and each element is equal, then the two
-  sequences are equal */
-  lemma lemma_seq_extensionality<T>(s: seq<T>, t: seq<T>)
-    requires |s| == |t|
-    requires forall i | 0 <= i < |s| :: s[i] == t[i]
-    ensures s == t
   {
   }
 
@@ -853,35 +511,7 @@ module Seq {
   {
     lemma_seq_slice_slice(ar[..], i, j, k, l);
   }
-
-  /* if two sequences have the same elements in a certain interval
-  the subsequences over that interval are equal */
-  lemma lemma_seq_extensionality_slice<T>(s: seq<T>, t: seq<T>, a: int, b: int)
-    requires 0 <= a <= b <= |s|
-    requires b <= |t|
-    requires forall i | a <= i < b :: s[i] == t[i]
-    ensures s[a..b] == t[a..b]
-  {
-  }
-
-  // fills the sequence with n identical elements
-  function method {:opaque} fill<T>(n: int, t: T): (res: seq<T>)
-    requires n >= 0
-    ensures |res| == n
-    ensures forall i | 0 <= i < n :: res[i] == t
-  {
-    if n == 0 then [] else fill(n-1, t) + [t]
-  }
-
-  /* concatenating two sequences and then taking a slice starting from an index 
-  that is greater than the first sequence is the same as taking a slice from the 
-  second sequence */
-  lemma sum_slice_second<T>(a: seq<T>, b: seq<T>, i: int, j: int)
-    requires |a| <= i <= j <= |a| + |b|
-    ensures (a+b)[i..j] == b[i-|a| .. j-|a|]
-  {
-  }
-
+  
   // converts a map to a sequence
   function method {:opaque} convert_map_to_seq<T>(n:int, m:map<int, T>): seq<T>
     requires n >= 0;
